projectVampire/dafny/insertionSort.dfy
@@ -99,7 +99,7 @@ class Blood{
 
 predicate Sorted(arr: array<int>, start:int, end:int)
 requires arr != null;
-requires 0<=start<arr.Length;
+requires 0<=start<=arr.Length;
 requires end <= arr.Length;
 //requires forall x :: 0 <= x < arr.Length ==> arr[x] != null;
 reads arr;
@@ -167,17 +167,24 @@ reads arr2[..];
 method insertionSort(toSort: array<int>, toMatch: array<Blood>)
 requires toSort != null;
 requires toMatch != null;
+requires forall x :: 0<=x<toMatch.Length ==> toMatch[x]!=null
 requires toSort.Length == toMatch.Length;
 //requires forall x :: 0 <= x < toSort.Length ==> toSort[x] != null
 requires forall x,y ::0 <= x < toSort.Length && 0 <= y < toMatch.Length && x == y  && toMatch[y] != null ==> toMatch[y].expiry_time == toSort[x];
 
-requires toSort.Length > 1;
 ensures Sorted(toSort,0,toSort.Length-1);
 ensures multiset(toSort[..]) == multiset(old(toSort[..]));
+ensures multiset(toMatch[..])==multiset(old(toMatch[..]))
 ensures forall x, y :: 0 <= x < toSort.Length && 0 <= y < toMatch.Length && x == y && toMatch[y] != null ==> toMatch[y].expiry_time == toSort[x];
+ensures forall x :: 0<=x<toMatch.Length ==> toMatch[x]!=null
 modifies toSort;
 modifies toMatch;
 {
+    if (toSort.Length<2)
+    {
+        // A length 0 or 1 array is already sorted
+        return;
+    }
     var start := 1;
     while (start < toSort.Length)
     invariant 1 <= start <= toSort.Length;
@@ -185,6 +192,7 @@ modifies toMatch;
     invariant multiset(toSort[..]) == multiset(old(toSort[..])); // keep array the same
     invariant multiset(toMatch[..]) == multiset(old(toMatch[..]));
     invariant forall x, y :: 0 <= x < toMatch.Length && 0 <= toSort.Length && x == y && toMatch[x] != null ==> toSort[y] == toMatch[x].expiry_time;
+    invariant forall x :: 0<=x<toMatch.Length ==> toMatch[x]!=null
     //invariant Matching(toSort, toMatch);
     //invariant forall x :: 0 <= x < toSort.Length ==> toSort[x] != null
     //invariant forall x :: 0 <= x < toSort.Length 
@@ -193,26 +201,28 @@ modifies toMatch;
         while (end >= 1 && toSort[end-1] > toSort[end])
         invariant 0 <= end <= start; // end is within limits
         invariant multiset(toSort[..]) == multiset(old(toSort[..])); // array stays the same
-	invariant multiset(toMatch[..]) == multiset(old(toMatch[..]));
-	//invariant Matching(toSort, toMatch);
-	//invariant forall i :: 0 <= i < toSort.Length ==> toSort[i] != null;
+        invariant multiset(toMatch[..]) == multiset(old(toMatch[..]));
+        //invariant Matching(toSort, toMatch);
+        //invariant forall i :: 0 <= i < toSort.Length ==> toSort[i] != null;
         invariant forall i, j :: (0 <= i <= j <= start && j != end) ==> toSort[i] <= toSort[j]; // all values less than start are sorted
         //invariant forall i :: (0 <= i <= start && i != end && toMatch[i] != null) ==> toSort[i] == toMatch[i].expiry_time;
         invariant forall x, y :: 0 <= x < toMatch.Length && 0 <= toSort.Length && x == y && toMatch[x] != null ==> toSort[y] == toMatch[x].expiry_time;
-	{
-           	var temp := toSort[end-1];
-           	toSort[end-1] := toSort[end];
-            	toSort[end] := temp;
-		
-	    	var temp2 := toMatch[end-1];
-	    	toMatch[end-1] := toMatch[end];
-	    	toMatch[end] := temp2;
-		
-		end := end -1;
-		
+        invariant forall x :: 0<=x<toMatch.Length ==> toMatch[x]!=null
+        {
+            var temp := toSort[end-1];
+            toSort[end-1] := toSort[end];
+                toSort[end] := temp;
+        
+            var temp2 := toMatch[end-1];
+            toMatch[end-1] := toMatch[end];
+            toMatch[end] := temp2;
+        
+        end := end -1;
+        
         }
         start := start + 1;
     }
+    
 }
 
 
